chore: import changes to framework

SSA/Core/Framework.lean
@@ -141,6 +141,13 @@ Another option, which would be more complicated, but correct by construction, is
 impurely.
 -/
 
+class DialectPrint (d : Dialect) where
+  printOpName : d.Op → String
+  printTy : d.Ty → String
+  printAttributes : d.Op → String
+  printDialect : String
+  printReturn : d.Ty → String
+  printFunc : d.Ty → String
 
 /- # Datastructures -/
 section DataStructures
@@ -178,6 +185,21 @@ inductive Lets (Γ_in : Ctxt d.Ty) (eff : EffectKind) :
   | nil : Lets Γ_in eff Γ_in
   | var (body : Lets Γ_in eff Γ_out) (e : Expr d Γ_out eff t) : Lets Γ_in eff (Γ_out.snoc t)
 
+/-- `Zipper d Γ_in eff Γ_mid ty` represents a particular position in a program, by storing the
+`Lets` that come before this position separately from the `Com` that represents the rest.
+Thus, `Γ_in` is the context of the program as a whole, while `Γ_mid` is the context at the
+current position.
+
+While technically the position is in between two let-bindings, by convention we say that the first
+binding of `top : Lets ..` is the current binding of a particular zipper. -/
+structure Zipper (Γ_in : Ctxt d.Ty) (eff : EffectKind) (Γ_mid : Ctxt d.Ty) (ty : d.Ty) where
+  /-- The let-bindings at the top of the zipper -/
+  top : Lets d Γ_in eff Γ_mid
+  /-- The program at the bottom of the zipper -/
+  bot : Com d Γ_mid eff ty
+
+
+
 /-! ### Repr instance -/
 section Repr
 open Std (Format)
@@ -191,6 +213,14 @@ private def Format.parenIfNonempty (l : String) (r : String) (separator : Format
   | [] => ""
   | _  =>  l ++ (Format.joinSep xs separator) ++ r
 
+/-- Parenthesize and separate with 'separator' if the list is nonempty, and return
+the "()" if the list is empty. -/
+private def Format.parenIfNonemptyForPrint (l : String) (r : String) (separator : Format)
+    (xs : List Format) : Format :=
+  match xs with
+  | [] => "() "
+  | _  =>  l ++ (Format.joinSep xs separator) ++ r
+
 /-- Format a sequence of types as `(t₁, ..., tₙ)`. Will always display parentheses. -/
 private def formatTypeTuple [Repr Ty] (xs : List Ty) : Format :=
   "("  ++ Format.joinSep (xs.map (fun t => Repr.reprPrec t 0)) ", " ++ ")"
@@ -199,6 +229,17 @@ private def formatTypeTuple [Repr Ty] (xs : List Ty) : Format :=
 private def formatArgTuple [Repr Ty] {Γ : List Ty}
     (args : HVector (fun t => Var Γ₂ t) Γ) : Format :=
   Format.parenIfNonempty "(" ")" ", " (formatArgTupleAux args) where
+  formatArgTupleAux [Repr Ty] {Γ : List Ty} (args : HVector (fun t => Var Γ₂ t) Γ) : List Format :=
+    match Γ with
+    | .nil => []
+    | .cons .. =>
+      match args with
+      | .cons a as => (repr a) :: (formatArgTupleAux as)
+
+/-- Format a tuple of arguments as `a₁, ..., aₙ`. -/
+private def formatArgTupleForPrint [Repr Ty] {Γ : List Ty}
+    (args : HVector (fun t => Var Γ₂ t) Γ) : Format :=
+  Format.parenIfNonemptyForPrint "(" ")" ", " (formatArgTupleAux args) where
   formatArgTupleAux [Repr Ty] {Γ : List Ty} (args : HVector (fun t => Var Γ₂ t) Γ) : List Format :=
     match Γ with
     | .nil => []
@@ -303,6 +344,48 @@ instance : ToString (Expr d Γ eff t) where toString := Expr.toString
 
 end ToString
 
+/- # ToString instances for Com and Expr  -/
+section DialectPrint
+variable {d} [DialectPrint d][DialectSignature d] [Repr d.Op] [Repr d.Ty] [ToString d.Ty] [ToString d.Op]
+
+/-- Format a list of formal arguments as `(%0 : t₀, %1 : t₁, ... %n : tₙ)` -/
+partial def formatFormalArgListTuplePrint [ToString d.Ty] (ts : List d.Ty) : String :=
+  let args := (List.range ts.length).zip ts |>.map
+    (fun (i, t) => s!"%{i} : {DialectPrint.printTy t}")
+  "(" ++ String.intercalate ", " args ++ ")"
+
+-- Format a sequence of types as `(t₁, ..., tₙ)` using toString instances -/
+private def formatTypeTuplePrint [ToString d.Ty] (xs : List d.Ty) : String :=
+  "(" ++ String.intercalate ", " (xs.map DialectPrint.printTy) ++ ")"
+
+/--
+Converts an expression within a dialect to its MLIR string representation.
+Since MLIR generic syntax uses "" to denote operations, this function, this functions uses
+the DialectPrint typeclass of each dialect to print the various parts of an expressiom such as
+operation and types. Lastly, it arranges the expression printing according to MLIR syntax.
+-/
+partial def Expr.toPrint [ToString d.Op] : Expr d Γ eff t → String
+  | Expr.mk (op : d.Op) _ _ args _regArgs =>
+    let outTy : d.Ty := DialectSignature.outTy op
+    let argTys := DialectSignature.sig op
+    s!"\"{DialectPrint.printOpName op}\"{formatArgTupleForPrint args}{DialectPrint.printAttributes op} : {formatTypeTuplePrint argTys} -> ({DialectPrint.printTy outTy})"
+
+/-- This function recursivly converts the body of a `Com` into its string representation.
+Each bound variable is printed with its index and corresponding expression. -/
+partial def Com.ToPrintBody : Com d Γ eff t → String
+  | .ret v => s!"  \"{DialectPrint.printReturn t}\"({_root_.repr v }) : ({DialectPrint.printTy t}) -> ()"
+  | .var e body =>
+    s!"  %{_root_.repr <|(Γ.length)} = {Expr.toPrint e }" ++ "\n" ++
+    Com.ToPrintBody body
+
+/- `Com.toString` implements a toString instance for the type `Com`.  -/
+partial def Com.toPrint (com : Com d Γ eff t) : String :=
+   "builtin.module { \n"
+  ++ DialectPrint.printFunc t ++ ((formatFormalArgListTuplePrint Γ.toList)) ++ ":" ++ "\n"
+  ++ (Com.ToPrintBody com) ++
+   "\n }"
+
+end DialectPrint
 /-! ### DecidableEq instance -/
 --TODO: this should be derived later on when a derive handler is implemented
 mutual -- DecEq
@@ -420,6 +503,21 @@ theorem Com.recAux'_eq :
   induction com <;> simp [recAux', *]
 
 end Rec
+
+
+/-- Alternative recursion principle for known-pure `Com`s.
+
+NOTE: this can now be achieved through `Com.rec'` direclty;
+`recPure` is deprecated and will be removed soon. -/
+-- TODO: eventually remove this
+@[elab_as_elim, deprecated Com.rec' (since := "")]
+def Com.recPure {t} {motive : ∀ {Γ t}, Com d Γ .pure t → Sort u}
+    (ret : ∀ {Γ}, (v : Var Γ t) → motive (Com.ret v))
+    (var : ∀ {Γ} {u : d.Ty},
+      (e : Expr d Γ .pure u) → (body : Com d (Γ.snoc u) .pure t) →
+        motive body → motive (Com.var e body))
+    {Γ} (com : Com d Γ .pure t) : motive com :=
+  com.rec' (motive := motive) ret var
 
 def Expr.op {Γ : Ctxt d.Ty} {eff : EffectKind} {ty : d.Ty} (e : Expr d Γ eff ty) : d.Op :=
   Expr.casesOn e (fun op _ _ _ _ => op)
@@ -539,6 +637,29 @@ section Lemmas
     returnVar (var (d:=d) (eff:=eff) e body) = body.returnVar := by
   simp [returnVar]
 
+/-!
+### `Lets.addComToEnd` and `Com.toLets`
+-/
+
+/-- Add a `Com` to the end of a sequence of lets -/
+def Lets.addComToEnd {Γ_out} {eff} (lets : Lets d Γ_in eff Γ_out) :
+      (com : Com d Γ_out eff ty) → Lets d Γ_in eff com.outContext
+  | Com.ret _       => lets
+  | Com.var e body => addComToEnd (Lets.var lets e) body
+
+/-- The let-bindings of a program -/
+def Com.toLets (com : Com d Γ eff t) : Lets d Γ eff com.outContext :=
+  Lets.nil.addComToEnd com
+
+section Lemmas
+
+@[simp] lemma Lets.addComToEnd_ret {lets : Lets d Γ_in eff Γ_out} :
+    addComToEnd lets (.ret v : Com d Γ_out eff t) = lets             := by simp [addComToEnd]
+@[simp] lemma Lets.addComToEnd_var {lets : Lets d Γ_in eff Γ_out} {com : Com d _ eff t} :
+    addComToEnd lets (Com.var e com) = addComToEnd (lets.var e) com := by simp [addComToEnd]
+
+@[simp] lemma Com.toLets_ret : toLets (ret v : Com d Γ eff t) = .nil := by simp [toLets]
+
 end Lemmas
 
 /-!
@@ -593,6 +714,12 @@ the congruence, you can do: `rw [← Lets.denotePure]; congr`
 -/
 @[simp] abbrev Lets.denotePure [DialectSignature d] [DialectDenote d] :
     Lets d Γ₁ .pure Γ₂ → Valuation Γ₁ → Valuation Γ₂ := Lets.denote
+
+/-- The denotation of a zipper is a composition of the denotations of the constituent
+`Lets` and `Com` -/
+def Zipper.denote (zip : Zipper d Γ_in eff Γ_out ty) (V_in : Valuation Γ_in) :
+    eff.toMonad d.m ⟦ty⟧ :=
+  (zip.top.denote V_in) >>= zip.bot.denote
 
 section Unfoldings
 
@@ -700,6 +827,25 @@ section Lemmas
 @[simp] lemma Lets.denote_var {lets : Lets d Γ_in eff Γ_out} {e : Expr d Γ_out eff t} :
     (lets.var e).denote = fun V_in => lets.denote V_in >>= e.denote :=
   rfl
+
+
+
+@[simp] lemma Lets.denote_addComToEnd
+    {lets : Lets d Γ_in eff Γ_out} {com : Com d Γ_out eff t} :
+    Lets.denote (lets.addComToEnd com) = fun V => (do
+        let Vlets ← lets.denote V
+        let Vbody ← com.denoteLets Vlets
+        return Vbody
+      ) := by
+  induction com
+  case ret => simp [Com.denoteLets]
+  case var ih => simp [addComToEnd, ih, denote_var]
+
+@[simp] lemma Com.denoteLets_ret : (.ret v : Com d Γ eff t).denoteLets = fun V => pure V := by
+  funext V; simp [denoteLets]
+
+theorem Com.denoteLets_eq {com : Com d Γ eff t} : com.denoteLets = com.toLets.denote := by
+  simp only [toLets]; induction com using Com.rec' <;> simp [Lets.denote_var]
 
 end Lemmas
 
@@ -938,6 +1084,22 @@ section Lemmas
     (com.castPureToEff eff).size = com.size := by
   induction com using Com.rec' <;> simp [*]
 
+@[simp] lemma Lets.addComToEnd_castPureToEff {lets : Lets d Γ_in .pure Γ_out}
+    {com : Com d Γ_out .pure ty} :
+    (lets.castPureToEff eff).addComToEnd (com.castPureToEff eff)
+    = cast (by simp) ((lets.addComToEnd com).castPureToEff eff) := by
+  induction com using Com.rec'
+  case ret => simp
+  case var ih =>
+    simp only [Com.castPureToEff_var, Com.outContext_var, addComToEnd_var,
+      ← Lets.castPureToEff_var, ih]
+
+@[simp] lemma Com.toLets_castPureToEff {com : Com d Γ .pure ty} :
+    (com.castPureToEff eff).toLets = cast (by simp) (com.toLets.castPureToEff eff) := by
+  unfold toLets
+  rw [show (Lets.nil : Lets d Γ eff Γ) = (Lets.nil.castPureToEff eff) from rfl,
+    Lets.addComToEnd_castPureToEff]
+
 @[simp] lemma Com.returnVar_castPureToEff {com : Com d Γ .pure ty} :
     (com.castPureToEff eff).returnVar = com.returnVar.castCtxt (by simp) := by
   induction com using Com.rec' <;> simp_all
@@ -959,6 +1121,14 @@ section Lemmas
   funext V
   induction com using Com.rec'
   · rfl
+  · simp [*]; rfl
+
+@[simp] lemma Com.denoteLets_castPureToEff {com : Com d Γ .pure ty} :
+    denoteLets (com.castPureToEff eff)
+    = fun V => pure (com.denoteLets V |>.comap fun _ v => v.castCtxt (by simp)) := by
+  funext V
+  induction com using Com.rec'
+  · simp
   · simp [*]; rfl
 
 end Lemmas
@@ -1018,6 +1188,97 @@ theorem Expr.denote_toPure? {e : Expr d Γ eff ty} {e': Expr d Γ .pure ty}
   obtain ⟨h_pure, rfl⟩ : ∃ (h : e.HasPureOp), e.toPure h = e' := by
     simpa [toPure?] using he
   rw [denote_pure, EffectKind.pure_pure, ← map_pure, Expr.pure_denoteOp_toPure, denote_unfold]
+/-!
+## Combining `Lets` and `Com`
+
+Various machinery to combine `Lets` and `Com`s in various ways.
+
+-/
+
+-- TODO: this doesn't morally fit here, but we can't yoink it up, figure out what to do
+/-- Convert a `Com` into a `FlatCom` -/
+def Com.toFlatCom {t : d.Ty} (com : Com d Γ .pure t) : FlatCom d Γ .pure com.outContext t :=
+  ⟨com.toLets, com.returnVar⟩
+
+/-- Recombine a zipper into a single program by adding the `lets` to the beginning of the `com` -/
+def Zipper.toCom (zip : Zipper d Γ_in eff Γ_mid ty) : Com d Γ_in eff ty :=
+  go zip.top zip.bot
+  where
+    go : {Γ_mid : _} → Lets d Γ_in eff Γ_mid → Com d Γ_mid eff ty → Com d Γ_in eff ty
+      | _, .nil, com          => com
+      | _, .var body e, com  => go body (.var e com)
+
+/-- Add a `Com` directly before the current position of a zipper, while reassigning every
+occurence of a given free variable (`v`) of `zip.com` to the output of the new `Com`  -/
+def Zipper.insertCom (zip : Zipper d Γ_in eff Γ_mid ty) (v : Var Γ_mid newTy)
+    (newCom : Com d Γ_mid eff newTy) : Zipper d Γ_in eff newCom.outContext ty :=
+  let newTop := zip.top.addComToEnd newCom
+  --  ^^^^^^ The combination of the previous `top` with the `newCom` inserted
+  let newBot := zip.bot.changeVars <| newCom.outContextHom.with v newCom.returnVar
+  --  ^^^^^^ Adjust variables in `bot` to the intermediate context of the new zipper --- which is
+  --         `newCom.outContext` --- while also reassigning `v`
+  ⟨newTop, newBot⟩
+
+/-- Add a pure `Com` directly before the current position of a possibly impure
+zipper, while r eassigning every occurence of a given free variable (`v`) of
+`zip.com` to the output of the new `Com`
+
+This is a wrapper around `insertCom` (which expects `newCom` to have the same effect as `zip`)
+and `castPureToEff` -/
+def Zipper.insertPureCom (zip : Zipper d Γ_in eff Γ_mid ty) (v : Var Γ_mid newTy)
+    (newCom : Com d Γ_mid .pure newTy) : Zipper d Γ_in eff newCom.outContext ty :=
+  (by simp : (newCom.castPureToEff eff).outContext = newCom.outContext)
+    ▸ zip.insertCom v (newCom.castPureToEff eff)
+
+/-! simp-lemmas -/
+section Lemmas
+
+@[simp] lemma Zipper.toCom_nil {com : Com d Γ eff ty} : Zipper.toCom ⟨.nil, com⟩ = com := rfl
+@[simp] lemma Zipper.toCom_var {lets : Lets d Γ_in eff Γ_mid} :
+    Zipper.toCom ⟨Lets.var lets e, com⟩ = Zipper.toCom ⟨lets, Com.var e com⟩ := rfl
+
+@[simp] theorem Zipper.denote_toCom [LawfulMonad d.m] (zip : Zipper d Γ_in eff Γ_mid ty) :
+    zip.toCom.denote = zip.denote := by
+  rcases zip with ⟨lets, com⟩
+  funext Γv; induction lets <;> simp [Lets.denote, Zipper.denote, *]
+
+@[simp] lemma Zipper.denote_mk {lets : Lets d Γ_in eff Γ_out} {com : Com d Γ_out eff ty} :
+    denote ⟨lets, com⟩ = fun V => (lets.denote V) >>= com.denote := rfl
+
+theorem Zipper.denote_insertCom {zip : Zipper d Γ_in eff Γ_mid ty₁}
+    {newCom : Com d _ eff newTy} [LawfulMonad d.m] :
+    (zip.insertCom v newCom).denote = (fun (V_in : Valuation Γ_in) => do
+      let V_mid ← zip.top.denote V_in
+      let V_newMid ← newCom.denoteLets V_mid
+      zip.bot.denote
+        (V_newMid.comap <| newCom.outContextHom.with v newCom.returnVar)
+      ) := by
+  funext V
+  simp [insertCom, Com.denoteLets_eq]
+
+/-- Casting the intermediate context is not relevant for the denotation -/
+@[simp] lemma Zipper.denoteLets_eqRec_Γ_mid {zip : Zipper d Γ_in eff Γ_mid ty}
+    (h : Γ_mid = Γ_mid') :
+    denote (h ▸ zip) = zip.denote := by
+  subst h; rfl
+
+theorem Zipper.denote_insertPureCom {zip : Zipper d Γ_in eff Γ_mid ty₁}
+    {newCom : Com d _ .pure newTy} [LawfulMonad d.m] :
+    (zip.insertPureCom v newCom).denote = (fun (V_in : Valuation Γ_in) => do
+      let V_mid ← zip.top.denote V_in
+      zip.bot.denote
+        ((Com.denoteLets newCom V_mid).comap <| newCom.outContextHom.with v newCom.returnVar)
+      ) := by
+  have (V_mid) (h : Com.outContext (Com.castPureToEff eff newCom) = Com.outContext newCom) :
+      ((Com.denoteLets newCom V_mid).comap fun x v => v.castCtxt h).comap
+        (newCom.castPureToEff eff).outContextHom
+      = (Com.denoteLets newCom V_mid).comap newCom.outContextHom := by
+    funext t' ⟨v', hv'⟩
+    simp only [Com.outContextHom, Com.outContextDiff, Com.size_castPureToEff]
+    rfl
+  funext V; simp [insertPureCom, denote_insertCom, Valuation.comap, this]
+
+end Lemmas
 
 /-!
 ### Semantic preservation of `Zipper.insertPureCom`
